$$B(r,\theta) = |\mathbf{B}| = |\frac{-μ_0m}{4π}\Big(\frac{-2m}{4π}\cos(θ)\widehat {\boldsymbol r}+\frac{-m}{4π}\sin(θ)\widehat {\boldsymbol θ}\Big)| \=|\frac{-μ_0m}{4π}\Big(\frac{-2m}{4π}\cos(θ)\widehat {\boldsymbol r}+\frac{-m}{4π}\sin(θ)\widehat {\boldsymbol θ}\Big)| \=|\frac{-μ_0m}{4π}\Big(\Big(\frac{-2m}{4π}\cos(θ)\widehat {\boldsymbol r}+\frac{-m}{4π}\sin(θ)\widehat {\boldsymbol θ}\Big)| \=|\frac{-μ_0m}{4π}\Big(\Big(\frac{-2m}{4π}\cos(θ)\widehat {\boldsymbol r}+\frac{-m}{4π}\sin(θ)\widehat {\boldsymbol θ}\Big)| \=|\frac{-μ_0m}{4π}\Big(\Big(\frac{-2m}{4π}\cos(θ)\widehat {\boldsymbol r}+\frac{-m}{4π}\sin(θ)\widehat {\boldsymbol θ}\Big)| \=|\frac{-μ_0m}{4π}\Big(\Big(\frac{-2m}{4π}$$